model reimplemented

flp.v
@@ -1,210 +1,200 @@
 (** FLP Impossibility Proof **)
 (** Made after original paper http://cs-www.cs.yale.edu/homes/arvind/cs425/doc/fischer.pdf **) 
+(** Also see an awesome blogpost http://the-paper-trail.org/blog/a-brief-tour-of-flp-impossibility/ **)
 
+Require Import Arith.
+Require Import List.
 
-Require Export BinPos.
-Require Export List.
-Require Export Coq.Arith.Compare_dec.
-Require Export Coq.Lists.List.
-Require Export Coq.PArith.Pnat.
-Require Export Coq.Lists.ListSet.
-Require Export Coq.Classes.EquivDec.
-Require Export Coq.Vectors.VectorDef.
-Require Export Coq.Vectors.Fin.
-Require Export Setoid.
-
-
-Local Open Scope nat_scope.
+Set Implicit Arguments.
 Import ListNotations.
-Local Open Scope list_scope.
 
 
-(** Each process p has a one-bit input register x, an output register y with 
-values in (b, 0, 1), so (b, f, t) **)
-Inductive Register :Type :=
-  | b
-  | fval
-  | tval.
+Definition Binary := bool.
 
 
-Definition InternalState:Type := nat.
+Inductive Process: Set := 
+| FinishedProcess: Binary -> Process
+| FailedProcess
+| proceed: nat -> Process. 
 
-Definition MessageValue:Type := nat.
+Definition failedProcess(p:Process):bool := match p with
+| FailedProcess => true
+| _ => false
+end.
 
-Theorem mv_eq_dec : forall x y:MessageValue, {x = y} + {x <> y}.
-Proof. intros. auto with *. Qed.
-
-Inductive Message:Type := 
-| emptyMessage
-| messageValue: MessageValue -> Message.
-
-Parameter numOfProcesses:nat.
-Hypothesis np2: numOfProcesses >= 2.
-
-Definition ProcessId := Fin.t numOfProcesses.
-
-Definition Event : Type := prod ProcessId MessageValue.
-
-Record Process : Type := {
-   inputRegister : Register;
-   outputRegister : Register;
-   internalState : InternalState;
-   transitionFunction: InternalState -> Message -> prod InternalState (list Event);
-   messagesBuffer : set MessageValue 
-}.
-
-Definition updateMsgBuf (p:Process)(mb:set MessageValue):Process := 
-({|inputRegister := p.(inputRegister); outputRegister := p.(outputRegister);
-   internalState := p.(internalState); transitionFunction := p.(transitionFunction);
-   messagesBuffer := mb |}).
-
-Definition updateState (p:Process)(msg:Message) : prod Process (list Event):= 
-let (newState, evts) := p.(transitionFunction) p.(internalState) msg in 
-pair ({|inputRegister := p.(inputRegister); outputRegister := p.(outputRegister);
-   internalState := newState; transitionFunction := p.(transitionFunction);
-   messagesBuffer := p.(messagesBuffer) |}) evts.
-
-Definition removeMsg (p:Process)(mv:MessageValue):Process := 
-   updateMsgBuf p (remove mv_eq_dec  mv p.(messagesBuffer)).
- 
-
-
-Definition decisionState (p:Process) : Prop :=
-match outputRegister p with
-|b => False
-|_ => True
+Definition finishedIn(b:Binary)(p:Process):bool := match p with
+| FinishedProcess b => true
+| _ => false
 end.
 
 
-Definition Configuration:Type := Vector.t Process numOfProcesses.
-Parameter initialConfiguration : Configuration.
+Definition Configuration := list Process.
+
+Definition decidedValue(cfg:Configuration)(b:Binary):Prop := 
+In (FinishedProcess b) cfg.
+
+Definition decided(cfg:Configuration):Prop := decidedValue cfg true \/ decidedValue cfg false.
 
 
-Definition updateCfg (c:Configuration)(pid:ProcessId)(fn: Process -> Process) : Configuration :=
-replace c pid (fn (nth c pid)).
-
-Definition updateCfgWithEvents (c:Configuration)(pid:ProcessId)(fn: Process -> prod Process (list Event)) : prod (list Event) Configuration :=
-let (p, evs) := fn(nth c pid) in pair evs (replace c pid p).
-
-Definition send (cfg:Configuration) (pid:ProcessId) (mv: MessageValue)  : Configuration := 
-updateCfg cfg pid (fun p=> let pmsgs : set MessageValue  := messagesBuffer p in
-let newmsgs := set_add mv_eq_dec mv pmsgs in updateMsgBuf p newmsgs).
-
-
-Import VectorNotations.
-
-(** todo: prove the lemma **)
-Lemma cfg_replace_replaced: forall pid p (c:Configuration), nth (replace c pid p) pid = p.
-
-(** todo: prove the lemma **)
-Lemma cfg_replace_comm: forall pid1 pid2 p1 p2 (c:Configuration), pid1 <> pid2 -> replace (replace c pid1 p1) pid2 p2 = replace (replace c pid2 p2) pid1 p1.
-
-(** todo: prove the lemma **)
-Lemma updateCfg_comm: forall p1 p2 pid1 pid2 fn1 fn2 (c:Configuration), 
-pid1 <> pid2 -> p1 = fn1 c[@pid1] -> p2 = fn2 c[@pid2] -> updateCfg (updateCfg c pid1 fn1) pid2 fn2 = updateCfg (updateCfg c pid2 fn2) pid1 fn1.
-
-(** todo: prove the lemma **)
-Lemma send_length_comm: forall pid1 pid2 m c, pid1 <> pid2 -> send (send c pid2 m) pid1 m  = send (send c pid1 m) pid2 m.
-
-
-Definition getMessageAndUpdateProcess (choiceFn: set MessageValue -> Message)(p:Process) : prod Process (list Event) := 
-let (msg, pp) := (match choiceFn(messagesBuffer p) with
-| emptyMessage => pair emptyMessage p
-| messageValue mv =>  pair (messageValue mv) (removeMsg p mv)
-end) in updateState pp msg.
-
-(** receive with send **)
-Definition receive (choiceFn: set MessageValue -> Message) (cfg:Configuration) (pid:ProcessId) : prod (list Event) Configuration :=
-updateCfgWithEvents cfg pid (getMessageAndUpdateProcess choiceFn). 
+Axiom Corectness: forall cfg, ~(decidedValue cfg true /\ decidedValue cfg false).
 
 
 
+(** A particular execution, defined by a possibly infinite sequence of events from 
+a starting configuration C is called a schedule and the sequence of steps taken 
+to realise the schedule is a run **)
 
-Definition sendOut(c:Configuration)(evt:Event) : Configuration := send c (fst evt) (snd evt).
+Definition Schedule := list nat.
 
-
-Definition ChooseProcess := Configuration -> ProcessId.
-Variable chooseProcessImpl: ChooseProcess.
-
-Definition NonDeterministicChoice := set MessageValue -> Message.
-Variable ndChoiceImpl: NonDeterministicChoice.
-
-
-Definition auto_step (c:Configuration) : Configuration := 
-   let pid := chooseProcessImpl c in 
-   let (evts, c1) := receive ndChoiceImpl c pid in
-   List.fold_left sendOut evts c1.
+(** Configuration transition function **)
+Parameter eventFn : Configuration -> nat -> Configuration.
 
 
-Definition step (c:Configuration)(evt:Event) : Configuration := 
-   let pid := fst evt in 
-   let msgValue := snd evt in 
-   let (evts, c1) := receive (fun msgs => messageValue msgValue) c pid in
-   List.fold_left sendOut evts c1.
+(**Only one process changed 
+Axiom Step: **) 
 
 
-Definition Schedule := Configuration -> list Event.
-
-Definition Run (c:Configuration)(events: list Event):Configuration := List.fold_left step events c.
-
-
-Fixpoint disjoint (xl yl : list Event) :=
-  match xl with
-    | List.nil => True
-    | List.cons x xl =>  ~ List.In x yl /\ disjoint xl yl
-  end.
+(** There's no change in deciding value **)
+Axiom Termination: forall cfg b msg, decidedValue cfg b -> decidedValue (eventFn cfg msg) b.
 
 
- 
-(**
+Lemma Termination_1: forall cfg msg, decided cfg -> decided (eventFn cfg msg).
+Proof.
+intros.
+pose proof Termination as T.
+unfold decided.
+unfold decided in H.
+intuition.
+Qed.
 
-Testing code, to run with numOfProcesses defined, e.g. Definition numOfProcesses := 3.
 
-Definition e1:Event := pair (FS F1) (6:MessageValue).
-Definition e2:Event := pair (FS F1) (4:MessageValue).
-
-Lemma dj_ex_1 : disjoint (List.cons e1 List.nil) (List.cons e2 List.nil) -> True.
-Proof. trivial. Qed.
-
-Lemma dj_ex_2 : disjoint (List.cons e2 List.nil) (List.cons e2 List.nil) -> False.
-Proof. unfold disjoint. intros. intuition. Qed.
-
-**)
+Fixpoint run (cfg:Configuration)(s:Schedule): Configuration :=
+match s with
+| nil => cfg
+| cons msg t => eventFn (run cfg t) msg
+end.  
 
 
 
-(**
+Lemma Termination_2: forall cfg b s, decidedValue cfg b -> decidedValue (run cfg s) b.
+Proof.
+intros.
+pose proof Termination as T.
+unfold run.
+induction s.
+trivial.
+auto.
+Qed.
 
-LEMMA 1. Suppose that from some configuration C, the schedules s1, s2 lead 
-to configurations C1, C2, respectively. If the sets of processes taking steps 
-in C1 and C2, respectively, are disjoint, then s2 can be applied to C1 and s1 can be 
-applied to C2, and both lead to the same configuration Cf.
 
-**)
+(** An admissible run is one where at most one process is faulty 
+(and every message is eventually delivered) **)
+Definition admissible(cfg:Configuration)(s:Schedule): Prop := 
+    length (filter failedProcess (run cfg s)) <= 1.
 
-Lemma FLP_LEMMA1: forall c l1 l2, disjoint l1 l2 -> Run (Run c l1) l2 = Run (Run c l2) l1.
+
+Axiom OneFaultMax: forall (cfg:Configuration)(s:Schedule), admissible cfg s.
+
+
+(** We say that a run is deciding provided that some process eventually decides according 
+to the properties of consensus **)
+Definition deciding(cfg:Configuration)(s:Schedule): Prop := decided (run cfg s).
+
+Parameter InitialConfiguration: Configuration.
+
+
+Axiom InitialNoConsensus: ~decided InitialConfiguration.
+Axiom TrueReacheable: exists s1, decidedValue (run InitialConfiguration s1) true.
+Axiom FalseReacheable: exists s2, decidedValue (run InitialConfiguration s2) false.
+
+
+
+Definition univalent_true(cfg:Configuration):= (~ decided cfg) -> 
+(exists s1, decidedValue(run cfg s1) true) /\ ~(exists s2, decidedValue (run cfg s2) false).
+
+Definition univalent_false(cfg:Configuration):= (~ decided cfg) -> 
+(exists s1, decidedValue(run cfg s1) false) -> ~(exists s2, decidedValue (run cfg s2) true).
+
+Definition univalent(cfg:Configuration):= univalent_true cfg \/ univalent_false cfg.
+
+Definition bivalent(cfg:Configuration):= (~ decided cfg) ->
+((exists s1, decidedValue(run cfg s1) false) /\ 
+  (exists s2, decidedValue (run cfg s2) true)).
+
+Axiom ValuesReacheable: forall cfg, ~ decided cfg -> bivalent cfg \/ univalent cfg.
 
 
 
 
+Lemma BivNotUn: forall cfg, ~ decided cfg -> bivalent cfg -> ~ univalent cfg.
+Proof.
+intros.
+unfold bivalent in H0.
+unfold univalent.
+unfold univalent_true.
+unfold univalent_false.
+tauto.
+Qed.
 
-Definition decisionValues (c:Configuration) : prod Prop Prop  := let regs := map outputRegister c in
-pair (In fval regs) (In tval regs).
-
-Definition hasDecisionValue (c:Configuration) : Prop := let dv := decisionValues c in fst dv \/ snd dv. 
-Definition isZeroValent (c:Configuration) : Prop := let dv := decisionValues c in fst dv /\ ~ snd dv.
-Definition isOneValent (c:Configuration) : Prop := let dv := decisionValues c in fst dv /\ ~ snd dv.
-Definition isBivalent (c:Configuration) : Prop := let dv := decisionValues c in fst dv /\ snd dv.
 
 
+Theorem FLP_Lemma2: bivalent(InitialConfiguration).
+Proof.
+pose proof InitialNoConsensus as I.
+pose proof TrueReacheable as T.
+pose proof FalseReacheable as F.
+unfold bivalent.
+intuition.
+Qed.
 
-(** LEMMA 2. P has a bivalent initial configuration. **)
+Theorem FLP_Lemma3_pl: forall cfg s, bivalent cfg -> ~ decided cfg -> univalent_true (run cfg s) \/ univalent_false (run cfg s).
+Proof.
+unfold bivalent.
+unfold univalent_true.
+unfold univalent_false.
+intuition.
+pose proof Corectness as C.
+intuition.
+left.
+intuition.
+unfold decided in H1.
+intuition.
+destruct C.
 
-(** LEMMA 3. Let C be a bivalent configuration of P, and let e = (p, m) be an event 
-that is applicable to C. Let CE be the set of configurations reachable from C 
-without applying e, and let D = {e(E) = (e(E) | E belongs to CE and e is applicable to E). 
-Then, D contains a bivalent configuration. **)
+
+
+
+
+
+
+
+
+
+
+
+Theorem FLP_Lemma3: forall cfg, ~ decided cfg -> bivalent cfg -> exists s, bivalent (run cfg s).
+Proof.
+intros.
+pose proof ValuesReacheable as V.
+pose proof BivNotUn as B.
+
+
+
+
+
+
+
+
+
 
 (** THEOREM 1. No consensus protocol is totally correct in spite of one fault. **)
+
+Theorem FLP_main: forall m, exists s, length s > m -> ~(deciding InitialConfiguration s).
+Proof.
+intros.
+pose proof InitialNoConsensus as I.
+pose proof TrueReacheable as T.
+pose proof FalseReacheable as F.
+pose proof FLP_Lemma2 as FL2.
 
 
